src/tls/Encode.fst
@@ -9,6 +9,8 @@ module Encode
    16-01-04 verifies with temporary assumptions; TBC
  *)
 
+(* TODO: AR: Failed to verify implicits errors, 4 *)
+
 open FStar.Seq
 open Platform
 open Platform.Bytes
